thy/Bitmagic/NumberWangCaesar.thy
@@ -401,22 +401,7 @@ done
 
 declare word_upto.simps[simp del] 
 
-lemma word_upto_set_eq: "a \<le> b \<Longrightarrow> set (word_upto a b) = {a..b}"
-apply(induction a b rule: word_upto.induct)
-apply(case_tac "a = b")
-apply(simp)
-apply(subst word_upto.simps)
-apply(simp)
-apply(case_tac "a < b - 1")
-apply(subgoal_tac "{a..b} = insert b {a..b - 1}")
-apply(simp only:)
-defer
-apply(simp)
-apply(subst word_upto.simps)
-apply(subgoal_tac "a = b - 1")
-oops
-
-lemma word_upto_set_eq: "a \<le> b \<Longrightarrow> x \<in> set (word_upto a b) \<Longrightarrow> a \<le> x \<and> x \<le> b"
+lemma word_upto_set_eq2: "a \<le> b \<Longrightarrow> x \<in> set (word_upto a b) \<Longrightarrow> a \<le> x \<and> x \<le> b"
 apply(induction a b rule: word_upto.induct)
 apply(case_tac "a = b")
 apply(subst(asm) word_upto.simps)
@@ -427,19 +412,28 @@ apply(erule disjE)
 apply simp
 proof -
 	case goal1
-	from goal1(2,3) have "a \<le> b - 1" 
-	proof -
-	  have f1: "\<forall>w wa. (w\<Colon>'a word) - wa = word_of_int (uint w + - 1 * uint wa)"
-		by (simp add: word_arith_wis(2))
-	  hence f2: "b + - 1 = word_of_int (uint b + - 1 * uint (1\<Colon>'a word))"
-		by simp
-	  hence "\<not> - (1\<Colon>'a word) \<le> word_of_int (uint (word_of_int (uint b + - 1 * uint (1\<Colon>'a word))\<Colon>'a word) + - 1 * uint a)"
-		using f1 by (metis (no_types) add_diff_cancel diff_eq_diff_eq diff_right_commute eq_iff goal1(3) word_n1_ge)
-	  thus ?thesis
-		using f2 f1 by (metis (no_types) add_diff_cancel diff_right_commute goal1(2) leD not_leE sub_wrap word_less_minus_cancel word_sub_less_iff)
-	qed
-	from goal1(1)[OF this goal1(4)]
-	show ?case by (metis dual_order.trans goal1(2) goal1(3) less_imp_le measure_unat word_le_0_iff word_le_nat_alt)
-qed (* TODO: redo. maybe some b \<noteq> 0 would help *)
+	from goal1(2-3) have "b \<noteq> 0" by force
+	from goal1(2,3) have "a \<le> b - 1" by (metis `b \<noteq> 0` le_step_down_nat order_class.order.antisym unat_minus_one word_le_nat_alt) 
+	from goal1(1)[OF this goal1(4)] show ?case by (metis dual_order.trans goal1(2) goal1(3) less_imp_le measure_unat word_le_0_iff word_le_nat_alt)
+qed
+
+lemma word_upto_set_eq3: "a \<le> x \<and> x \<le> b \<Longrightarrow> x \<in> set (word_upto a b)"
+apply(induction a b rule: word_upto.induct)
+apply(case_tac "a = b")
+apply(subst word_upto.simps)
+apply(simp; force)
+apply(subst word_upto.simps)
+apply(simp)
+apply(case_tac "x = b")
+apply(simp;fail)
+proof -
+	case goal1
+	from goal1(2-4) have "b \<noteq> 0" by force
+	from goal1(2,4) have "x \<le> b - 1" by (metis `b \<noteq> 0` dual_order.antisym le_step_down_nat unat_minus_one word_le_nat_alt) 
+	from goal1(1) this show ?case by simp
+qed
+
+lemma word_upto_set_eq: "a \<le> b \<Longrightarrow> x \<in> set (word_upto a b) \<longleftrightarrow> a \<le> x \<and> x \<le> b"
+	using word_upto_set_eq3 word_upto_set_eq2 by metis
 
 end
